src/Lean/Elab/Do.lean
@@ -69,7 +69,7 @@ namespace Do
 
 /- A `doMatch` alternative. `vars` is the array of variables declared by `patterns`. -/
 structure Alt (σ : Type) :=
-(ref : Syntax) (vars : Array Name) (patterns : Array Syntax) (rhs : σ)
+(ref : Syntax) (vars : Array Name) (patterns : Syntax) (rhs : σ)
 
 /-
   Auxiliary datastructure for representing a `do` code block, and compiling "reassignments" (e.g., `x := x + 1`).
@@ -111,21 +111,21 @@ inductive Code
 | reassign     (xs : Array Name) (stx : Syntax) (cont : Code)
 /- The Boolean value in `params` indicates whether we should use `(x : typeof! x)` when generating term Syntax or not -/
 | joinpoint    (name : Name) (params : Array (Name × Bool)) (body : Code) (cont : Code)
-| action       (stx : Syntax) (cont : Code)
-| returnAction (stx : Syntax)
+| action       (stx : Syntax) (cont : Code) -- TODO: rename to `seq`?
+| returnAction (stx : Syntax)  -- TODO: rename to `result`?
 | «break»      (ref : Syntax)
 | «continue»   (ref : Syntax)
 | «return»     (ref : Syntax) (val : Syntax)
 /- Recall that an if-then-else may declare a variable using `optIdent` for the branches `thenBranch` and `elseBranch`. We store the variable name at `var?`. -/
 | ite          (ref : Syntax) (h? : Option Name) (optIdent : Syntax) (cond : Syntax) (thenBranch : Code) (elseBranch : Code)
-| «match»      (ref : Syntax) (discrs : Array Syntax) (type? : Option Syntax) (alts : Array (Alt Code))
+| «match»      (ref : Syntax) (discrs : Syntax) (optType : Syntax) (alts : Array (Alt Code))
 | jmp          (ref : Syntax) (jpName : Name) (args : Array Syntax)
 
 instance Code.inhabited : Inhabited Code :=
 ⟨Code.«break» (arbitrary _)⟩
 
 instance Alt.inhabited : Inhabited (Alt Code) :=
-⟨{ ref := arbitrary _, vars := #[], patterns := #[], rhs := arbitrary _ }⟩
+⟨{ ref := arbitrary _, vars := #[], patterns := arbitrary _, rhs := arbitrary _ }⟩
 
 /- A code block, and the collection of variables updated by it. -/
 structure CodeBlock :=
@@ -149,12 +149,10 @@ partial def toMessageDataAux (updateVars : MessageData) : Code → MessageData
 | Code.«continue» _         => "continue " ++ updateVars
 | Code.«return» _ _         => "return ... " ++ updateVars
 | Code.«match» _ ds t alts  =>
-  "match " ++ MessageData.joinSep (ds.toList.map MessageData.ofSyntax) ", " ++ " with " ++
+  "match " ++ ds ++ " with " ++
     alts.foldl
       (fun (acc : MessageData) (alt : Alt Code) =>
-        acc ++ Format.line ++ "| "
-        ++ MessageData.joinSep (alt.patterns.toList.map MessageData.ofSyntax) ", "
-        ++ " => " ++ toMessageDataAux alt.rhs)
+        acc ++ Format.line ++ "| " ++ alt.patterns ++ " => " ++ toMessageDataAux alt.rhs)
       Format.nil
 
 private def nameSetToArray (s : NameSet) : Array Name :=
@@ -444,6 +442,15 @@ unit ← `(PUnit.unit);
 let unit := unit.copyInfo ref;
 pure { c with code := Code.ite ref none mkNullNode cond (Code.«return» ref unit) c.code }
 
+def mkMatch (ref : Syntax) (discrs : Syntax) (optType : Syntax) (alts : Array (Alt CodeBlock)) : TermElabM CodeBlock := do
+-- nary version of homogenize
+let ws := alts.foldl (fun (ws : NameSet) alt => union ws alt.rhs.uvars) {};
+alts : Array (Alt Code) ← alts.mapM fun alt => do {
+  rhs ← extendUpdatedVars alt.rhs ws;
+  pure { ref := alt.ref, vars := alt.vars, patterns := alt.patterns, rhs := rhs.code : Alt Code }
+};
+pure { code := Code.«match» ref discrs optType alts, uvars := ws }
+
 /- Return a code block that executes `terminal` and then `k`.
    This method assumes `terminal` is a terminal -/
 def concat (terminal : CodeBlock) (k : CodeBlock) : TermElabM CodeBlock := do
@@ -499,13 +506,16 @@ letDecls.foldlM
 def getDoIdDeclVar (doIdDecl : Syntax) : Name :=
 (doIdDecl.getArg 0).getId
 
+def getPatternVarNames (pvars : Array PatternVar) : Array Name :=
+pvars.filterMap fun pvar => match pvar with
+  | PatternVar.localVar x => some x
+  | _ => none
+
 -- termParser >> leftArrow >> termParser >> optional (" | " >> termParser)
 def getDoPatDeclVars (doPatDecl : Syntax) : TermElabM (Array Name) := do
 let pattern := doPatDecl.getArg 0;
 patternVars ← getPatternVars pattern;
-pure $ patternVars.filterMap fun patternVar => match patternVar with
-  | PatternVar.localVar x => some x
-  | _ => none
+pure $ getPatternVarNames patternVars
 
 -- parser! "let " >> (doIdDecl <|> doPatDecl)
 def getDoLetArrowVars (doLetArrow : Syntax) : TermElabM (Array Name) := do
@@ -823,7 +833,19 @@ partial def toTerm : Code → M Syntax
   else do
     c ← liftM (expandReturnAction e);
     toTerm c
-| Code.«match» _ _ _ _    => liftM $ Macro.throwError Syntax.missing "WIP"
+| Code.«match» ref discrs optType alts => do
+  termSepAlts : Array Syntax ← alts.foldlM
+    (fun (termAlts : Array Syntax) alt => do
+      let termAlts := termAlts.push $ mkAtomFrom alt.ref "|";
+      rhs ← toTerm alt.rhs;
+      let termAlt  := mkNode `Lean.Parser.Term.matchAlt #[alt.patterns, mkAtomFrom alt.ref "=>", rhs];
+      let termAlts := termAlts.push termAlt;
+      pure termAlts)
+    #[];
+  let firstVBar     := termSepAlts.get! 0;
+  let termSepAlts   := mkNullNode $ termSepAlts.extract 1 termSepAlts.size;
+  let termMatchAlts := mkNode `Lean.Parser.Term.matchAlts #[mkNullNode #[firstVBar], termSepAlts];
+  pure $ mkNode `Lean.Parser.Term.«match» #[mkAtomFrom ref "match", discrs, optType, mkAtomFrom ref "with", termMatchAlts]
 
 def run (code : Code) (m : Syntax) (uvars : Array Name := #[]) (kind := Kind.regular) : MacroM Syntax := do
 term ← toTerm code { m := m, kind := kind, uvars := uvars };
@@ -984,8 +1006,27 @@ partial def doSeqToCode : List Syntax → M CodeBlock
         else do
           auxDo ← `(do let r ← $forInTerm; $uvarsTuple:term := r);
           doSeqToCode (getDoSeqElems (getDoSeq auxDo) ++ doElems)
-    else if k == `Lean.Parser.Term.doMatch then
-      throwError "WIP"
+    else if k == `Lean.Parser.Term.doMatch then do
+      /- Recall that
+         ```
+         def doMatchAlt   := sepBy1 termParser ", " >> darrow >> doSeq
+         def doMatchAlts  := parser! optional "| " >> sepBy1 doMatchAlt "|"
+         def doMatch      := parser! "match " >> sepBy1 matchDiscr ", " >> optType >> " with " >> doMatchAlts
+      -/
+      let ref       := doElem;
+      let discrs    := doElem.getArg 1;
+      let optType   := doElem.getArg 2;
+      let matchAlts := ((doElem.getArg 4).getArg 1).getArgs.getSepElems; -- Array of `doMatchAlt`
+      alts : Array (Alt CodeBlock) ←  matchAlts.mapM fun matchAlt => do {
+           let patterns := matchAlt.getArg 0;
+           pvars ← liftM $ getPatternsVars patterns.getArgs.getSepElems;
+           let vars := getPatternVarNames pvars;
+           let rhs  := matchAlt.getArg 2;
+           rhs ← withNewVars vars $ doSeqToCode (getDoSeqElems rhs);
+           pure { ref := matchAlt, vars := vars, patterns := patterns, rhs := rhs : Alt CodeBlock }
+        };
+      matchCode ← liftM $ mkMatch ref discrs optType alts;
+      concatWithRest matchCode
     else if k == `Lean.Parser.Term.doTry then
       throwError "WIP"
     else if k == `Lean.Parser.Term.doBreak then do
